Fix comments, better variables for example

trunk/examples/programs/chcToBoogie/pthread/01_inc-originalVarNames.bpl
@@ -9,36 +9,36 @@
 
 procedure I(value : int, m : int, loc1 : int, v1 : int, loc2 : int, v2 : int) returns ()
 {
-    var tmp1 : int;
-    var tmp2 : int;
-    var tmp3 : int;
+    var old_m : int;
+    var old_v : int;
+    var old_value : int;
 
     if (*) {
-        // Non-interference for lock();value:=v+1
-        assume (m == 0 && tmp2 == 1) && value == tmp3 + 1;
-        call I(tmp1, tmp2, loc1, v1, loc2, v2);
-        call I(tmp1, tmp2, loc1, v1, 1, tmp3);
-        call I(tmp1, tmp2, 1, tmp3, loc2, v2);
+        // Non-interference for value:=v+1;unlock()
+        assume m == 0 && old_m == 1 && value == old_v + 1;
+        call I(old_value, old_m, loc1, v1, loc2, v2);
+        call I(old_value, old_m, loc1, v1, 1, old_v);
+        call I(old_value, old_m, 1, old_v, loc2, v2);
     } else if (*) {
         // Symmetry
         call I(value, m, loc2, v2, loc1, v1);
     } else if (*) {
-        // Non-interference for v:=value;unlock()
-        assume (m == 1 && tmp2 == value) && tmp3 == 0;
-        call I(value, tmp3, 0, v1, loc2, v2);
-        call I(value, tmp3, loc1, v1, 0, v2);
-        call I(value, tmp3, loc1, v1, loc2, v2);
+        // Non-interference for lock();v:=value
+        assume m == 1 && old_m == 0;
+        call I(value, old_m, 0, v1, loc2, v2);
+        call I(value, old_m, loc1, v1, 0, v2);
+        call I(value, old_m, loc1, v1, loc2, v2);
     } else if (*) {
-        // Inductivity for v:=value;unlock()
-        assume ((m == 1 && tmp3 == 0) && loc1 == 1) && v1 == value;
-        call I(value, tmp3, 0, tmp2, loc2, v2);
+        // Inductivity for lock();v:=value
+        assume m == 1 && old_m == 0 && loc1 == 1 && v1 == value;
+        call I(value, old_m, 0, old_v, loc2, v2);
     } else if (*) {
         // Initial location
-        assume (m == 0 && loc1 == 0) && loc2 == 0;
+        assume m == 0 && loc1 == 0 && loc2 == 0;
     } else {
-        // Inductivity for lock();value:=v+1
-        assume ((m == 0 && value == v1 + 1) && tmp3 == 1) && loc1 == 2;
-        call I(tmp2, tmp3, 1, v1, loc2, v2);
+        // Inductivity for value:=v+1;unlock()
+        assume m == 0 && value == v1 + 1 && old_m == 1 && loc1 == 2;
+        call I(old_value, old_m, 1, v1, loc2, v2);
     }
 }
 
